Enum_Encode.sig
@@ -1,0 +1,23 @@
+signature Enum_Encode =
+sig
+ 
+ include Abbrev
+
+ type ('a,'b) fmap = ('a,'b) Redblackmap.dict
+
+ type logic_info 
+    = {enc : term,
+       dec : term,
+       enc_def : thm,
+       dec_def : thm,
+       dec_enc : thm}
+
+ val define_enum_encoding : hol_type -> logic_info
+
+  type enumMap = (hol_type, ((term * int) list * logic_info)) fmap
+
+  val base_enumMap : enumMap
+  val the_enumMap : unit -> enumMap
+  val insert_enum_type : hol_type * term list * logic_info -> unit
+
+end
