Enum_Encode.sml
@@ -1,0 +1,100 @@
+structure Enum_Encode :> Enum_Encode = 
+struct
+
+open HolKernel Parse boolLib bossLib MiscLib 
+
+local open splatTheory in end;
+
+ type logic_info 
+    = {enc : term,
+       dec : term,
+       enc_def : thm,
+       dec_def : thm,
+       dec_enc : thm}
+
+ type ('a,'b) fmap = ('a,'b) Redblackmap.dict
+
+structure Finmap = Redblackmap;
+
+type enumMap = (hol_type, ((term*int) list * logic_info)) fmap;
+
+(*---------------------------------------------------------------------------*)
+(* An enum type needs a formatting map from the enum constants to numbers.   *)
+(* The domain of the map is the name of the enum type.                       *)
+(*---------------------------------------------------------------------------*)
+
+val bool_logic_info = 
+    {enc = ``splat$enc_bool``,
+     dec = ``splat$dec_bool``,
+     enc_def = splatTheory.enc_bool_def,
+     dec_def = splatTheory.dec_bool_def,
+     dec_enc = splatTheory.dec_enc_bool}
+
+val base_enumMap : enumMap =
+  let open boolSyntax
+  in 
+    Finmap.fromList Type.compare [(Type.bool, ([(F,0), (T,1)], bool_logic_info))]
+  end;
+
+local
+    val emap = ref base_enumMap
+in 
+ fun the_enumMap() = !emap
+ fun insert_enum (k,v) = (emap := Finmap.insert (the_enumMap(), k,v))
+end
+
+fun insert_enum_type (ety,constrs,logic) =
+    insert_enum(ety,(map swap (enumerate 0 constrs),logic));
+
+fun define_enum_encoding ety =
+ let val etyName = fst(dest_type ety)
+     val clist = TypeBase.constructors_of ety
+     val eclist = map swap (enumerate 0 clist)
+     val teclist = map (I##numSyntax.term_of_int) eclist
+     val ename = "num_of_"^etyName
+     val dname = etyName^"_of_num"
+     val efnvar = mk_var(ename,ety --> numSyntax.num)
+     val dfnvar = mk_var(dname,numSyntax.num --> ety)
+     fun enc_clause (constr,itm) = mk_eq(mk_comb(efnvar,constr),itm)
+     val enc_clauses = map enc_clause teclist
+     val num_of_enum = TotalDefn.Define `^(list_mk_conj enc_clauses)`
+     val argvar = mk_var("n",numSyntax.num)
+     fun cond_of (c,n) x = mk_cond(mk_eq(argvar,n),c,x)
+     val (L,(b,_)) = front_last teclist
+     val body = itlist cond_of L b
+     val enum_of_num = TotalDefn.Define `^(mk_comb(dfnvar,argvar)) = ^body`
+     val n_of_e_const = mk_const(dest_var(efnvar))
+     val e_of_n_const = mk_const(dest_var(dfnvar))
+     val enumvar = mk_var("c",ety)
+     val stringvar = mk_var("s",stringSyntax.string_ty)
+     val encoderName = "enc_"^etyName
+     val decoderName = "dec_"^etyName
+     val encvar = mk_var(encoderName,ety --> stringSyntax.string_ty)
+     val decvar = mk_var(decoderName,stringSyntax.string_ty --> ety)
+     val encoder = TotalDefn.Define `^(mk_comb(encvar,enumvar)) = enc 1 (^n_of_e_const ^enumvar)`
+     val decoder = TotalDefn.Define `^(mk_comb(decvar,stringvar)) = ^e_of_n_const (dec ^stringvar)`
+     val encoder_const = mk_const(dest_var(encvar))
+     val decoder_const = mk_const(dest_var(decvar))
+     val inversion_goal = 
+       mk_forall(enumvar, 
+		 mk_eq(mk_comb(decoder_const,mk_comb(encoder_const, enumvar)),
+		       enumvar))
+     val inversion = 
+       prove (inversion_goal, 
+           Cases >> rw_tac std_ss 
+                      [encoder, decoder,splatTheory.dec_enc,
+                       num_of_enum, enum_of_num])
+     val coding = 
+        {enc = encoder_const,
+         dec = decoder_const,
+         enc_def = encoder,
+         dec_def = decoder,
+         dec_enc = inversion}
+ in
+   coding
+ end
+ handle e => raise wrap_exn "Enum_Encode" "define_enum_encoding" e
+
+end
+
+
