splatLib.sig
@@ -4,63 +4,46 @@ sig
 
   type regexp = Regexp_Type.regexp
 
-  type ('a,'b) fmap = ('a,'b) Redblackmap.dict
-
   datatype width
     = BITWIDTH of int
     | BYTEWIDTH of int
   
-  datatype endian = MSB | LSB
-  
-  datatype sign
-     = SIGNED of endian 
-     | UNSIGNED of endian
-  
-  datatype textrep = BIT | OCT | HEX | DEC;
-  
+  datatype atomic =
+     Interval of 
+       {span : IntInf.int * IntInf.int,
+        encoding : Regexp_Numerics.encoding,
+        endian : Regexp_Numerics.endian,
+        width  : width,
+        encoder : IntInf.int -> string,
+        decoder : string -> IntInf.int,
+        recog  : Regexp_Type.regexp}
+    | Enumset of 
+       {enum_type : hol_type,
+        constr_codes : (term * int) list,
+        logic : Enum_Encode.logic_info,
+        recog : Regexp_Type.regexp}
+    | StringLit of string
+    | Raw of width
+
+
   datatype format
-    = BINARY of sign * width
-    | TEXT of textrep * width
-    | ENUM of hol_type
+    = ATOM of atomic
+    | CONCAT of format list
+    | LIST of format
+    | ARRAY of format * int
+    | UNION of format * format
+    | PACKED of format list * width
 
-  datatype fieldval
-    = Num of Arbint.int * format 
-    | Interval of Arbint.int * Arbint.int * format
-    | Char of char * format
-    | Enumset of string * term list * format
-    | Raw of string * width
-    | Padding of width
-    | Packed of fieldval list;
-  
-  val format_of : fieldval -> format
 
-  type enumMap = (string, (term * int) list) fmap
-  val the_enumMap : unit -> enumMap
-  val insert_enum : string * (term * int) list -> unit
-  val define_enum_encoding : hol_type -> unit
-					       
-  type coding 
-      = {enc : term, 
-         dec : term,
-         enc_def : thm, 
-         dec_def : thm,
-         dec_enc : thm}
-
-  type codingMap = (format, coding) fmap
-  val the_codingMap : unit -> codingMap
-  val insert_coding : format * coding -> unit
-
-  val fieldval_to_tree : enumMap -> fieldval -> Regexp_Type.tree
-
-  type filter_info 
-       = {name: string,
-	  regexp : Regexp_Type.regexp,
-          encode_def : thm, 
-          decode_def : thm,
-          inversion : term,
-          correctness : term,
-          receiver_correctness : term,
-          implicit_constraints : thm option}
+  type filter_info
+   = {name : string,
+      regexp : Regexp_Type.regexp,
+      encode_def : thm, 
+      decode_def : thm,
+      inversion : term,
+      correctness : term,
+      receiver_correctness : term,
+      implicit_constraints : thm option};
 
   val filter_correctness : string * thm -> filter_info
 
